add proof of inconsistency

testsuite/tests/coqgen/cocti_examples.v
@@ -220,6 +220,23 @@ Definition Omega_False : M False :=
 
 Check Omega_False empty_env.
 
+(* Proof of inconsistency *)
+Definition extract_list [T] (r : W (list T)) : list T :=
+  if snd r is inl l then l else nil.
+
+Definition omega' : M (list bool) :=
+  do r_1 <- newref (ml_arrow ml_bool (ml_list ml_bool)) (fun x => Ret nil);
+  let delta _ : M (list bool) :=
+    (* produce an infinite stream by breaking the monad *)
+    do f <- getref _ r_1; fun e => Ret (true :: extract_list (f true e)) e in
+  do _ <- setref _ r_1 delta; delta true.
+
+Lemma contrad : let x := extract_list (omega' empty_env) in x = true :: x.
+Proof. done. Qed.
+
+Lemma inconsistency : False.
+Proof. move: contrad; by elim: (extract_list _) => //= a l IH [] ->. Qed.
+
 (* Evaluation loops *)
 (* Eval cbv in Omega empty_env. *)
 (* Use Scheme Equality, evaluation stops, but this is actually due to
